partial/LocalState.v
@@ -3,7 +3,7 @@
 Require Import List.
 Require Import Tactics.
 Require Import Coq.Program.Equality.
-Module State (mem : Memory).
+Module LocalState (mem : Memory).
 Import mem.
 
   
@@ -21,25 +21,25 @@ Definition state := nat.
 
 (** * Semantics *)
 
-Fixpoint eval (x: Expr) (q : state) : option nat * state :=
+Fixpoint eval (x: Expr) (q : state) : option (nat * state) :=
   match x with
-    | Val n => (Some n, q)
+    | Val n => Some (n, q)
     | Add x1 x2 => match eval x1 q with
-                   | (Some m, q') => match eval x2 q' with
-                                   | (Some n, q'') => (Some (m + n), q'')
-                                   | (None, q'') => (None, q'')
+                   | Some (m, q') => match eval x2 q' with
+                                   | Some (n, q'') => Some (m + n, q'')
+                                   | None => None
                                    end
-                   | (None, q') => (None, q')
+                   | None => None
                    end
-    | Throw => (None, q)
+    | Throw => None
     | Catch x h => match eval x q with
-                   | (Some n, q') => (Some n, q')
-                   | (None, q') => eval h q'
+                   | Some (n, q') => Some (n, q')
+                   | None => eval h q
                    end
-    | Get => (Some q, q)
+    | Get => Some (q, q)
     | Put x y => match eval x q with
-                 | (Some n, q') => eval y n
-                 | (None, q') => (None, q')
+                 | Some (n, q') => eval y n
+                 | None => None
                  end
   end.
 
@@ -72,28 +72,29 @@ Definition Han := option adr.
 
 Inductive Elem : Set :=
 | NUM : nat -> Elem
-| HAN : Code -> Han -> Elem.
+| HAN : Code -> Han -> state -> Elem.
 
 (** * Virtual Machine *)
 
 Inductive Conf : Type :=
 | conf : Code -> nat -> Han -> state -> Conf
-| fail : Han -> state -> Conf.
+| fail : Han -> Conf.
 
 
 Notation "⟨ x , y , z , q , s ⟩" := (conf x y z q, s).
-Notation "⟪ x , q , s ⟫" := (fail x q, s).
+Notation "⟪ x , s ⟫" := (fail x, s).
 
 Reserved Notation "x ==> y" (at level 80, no associativity).
 Inductive VM : Conf * Mem Elem -> Conf * Mem Elem -> Prop :=
 | vm_load n a c s q p : ⟨LOAD n c, a , p, q, s⟩ ==> ⟨c , n, p, q, s⟩ 
 | vm_add c s a r n q p : s[r]=  NUM n -> ⟨ADD r c, a , p, q, s⟩ ==> ⟨c , n + a, p, q, s⟩
 | vm_store c s a r q p : ⟨STORE r c, a, p, q, s⟩ ==> ⟨c , a, p, q, s[r:=NUM a]⟩
-| vm_throw a s q p : ⟨THROW, a, p, q, s⟩ ==> ⟪p, q, s⟫
-| vm_fail p p' s q c : s[p] = HAN c p' -> ⟪ Some p, q, s⟫ ==> ⟨c, 0, p', q, s⟩
-| vm_unmark p p' s a q c c' : s[p] = HAN c' p' ->
+| vm_throw a s q p : ⟨THROW, a, p, q, s⟩ ==> ⟪p, s⟫
+| vm_fail p p' s q c : s[p] = HAN c p' q -> ⟪ Some p, s⟫ ==> ⟨c, 0, p', q, s⟩
+| vm_unmark p p' s a q q' c c' : s[p] = HAN c' p' q' ->
                             ⟨UNMARK c, a, Some p, q, s⟩ ==> ⟨c, a, p', q, s⟩
-| vm_mark p r s a c c' q : ⟨MARK r c' c, a, p, q, s⟩ ==> ⟨c, a, Some r, q, s[r:= HAN c' p]⟩
+| vm_mark p r s a c c' q :
+    ⟨MARK r c' c, a, p, q, s⟩ ==> ⟨c, a, Some r, q, s[r:= HAN c' p q]⟩
 | vm_read a c s q p : ⟨READ c, a , p, q, s⟩ ==> ⟨c , q, p, q, s⟩
 | vm_write a c s q p : ⟨WRITE c, a , p, q, s⟩ ==> ⟨c , a, p, a, s⟩ 
 where "x ==> y" := (VM x y).
@@ -124,8 +125,8 @@ Theorem spec e r c a p s q :
   ⟨comp' e r c, a, p, q, s⟩
     =|>
     match eval e q with
-    | (Some n, q') => ⟨c , n, p, q', s⟩
-    | (None, q') => ⟪p, q', s⟫
+    | Some (n, q') => ⟨c , n, p, q', s⟩
+    | None => ⟪p, s⟫
     end.
 
 
@@ -147,8 +148,8 @@ Proof.
 
   begin
     match eval (Val n) q with
-    | (Some n', q') => ⟨c , n' ,p, q', s⟩
-    | (None, q') => ⟪p, q', s⟫
+    | Some (n', q') => ⟨c , n' ,p, q', s⟩
+    | None => ⟪p, s⟫
     end.
   = {auto}
       ⟨ c, n, p, q, s⟩.
@@ -160,42 +161,42 @@ Proof.
   
   begin
     match eval (Add e1 e2) q with
-    | (Some n, q') => ⟨c , n ,p, q', s⟩
-    | (None, q') => ⟪p, q', s⟫
+    | Some (n, q') => ⟨c , n ,p, q', s⟩
+    | None => ⟪p, s⟫
     end.
   = {auto}
     match eval e1 q with
-    | (Some n, q') => match eval e2 q' with
-                      | (Some n', q'') => ⟨c , n + n' , p, q'', s⟩
-                      | (None, q'') => ⟪p, q'', s⟫
+    | Some (n, q') => match eval e2 q' with
+                      | Some (n', q'') => ⟨c , n + n' , p, q'', s⟩
+                      | None => ⟪p, s⟫
                       end
-    | (None, q') => ⟪p, q', s⟫
+    | None => ⟪p, s⟫
     end.
   ≤ { auto }
     match eval e1 q with
-    | (Some n, q') => match eval e2 q' with
-                      | (Some n', q'') => ⟨c , n + n' ,p, q'', s[r:=NUM n]⟩
-                      | (None, q'') => ⟪p, q'', s[r:=NUM n]⟫
+    | Some (n, q') => match eval e2 q' with
+                      | Some (n', q'') => ⟨c , n + n' ,p, q'', s[r:=NUM n]⟩
+                      | None => ⟪p, s[r:=NUM n]⟫
                       end
-    | (None, q') => ⟪p, q', s⟫
+    | None => ⟪p, s⟫
     end.
   <== { apply vm_add }
       match eval e1 q with
-      | (Some n, q') => match eval e2 q' with
-                        | (Some n', q'') => ⟨ADD r c , n' ,p, q'', s[r:=NUM n]⟩
-                        | (None, q'') => ⟪p, q'', s[r:=NUM n]⟫
+      | Some (n, q') => match eval e2 q' with
+                        | Some (n', q'') => ⟨ADD r c , n' ,p, q'', s[r:=NUM n]⟩
+                        | None => ⟪p, s[r:=NUM n]⟫
                         end
-      | (None, q') => ⟪p, q', s⟫
+      | None => ⟪p, s⟫
       end.
   <|= {apply IHe2}
       match eval e1 q with
-      | (Some n, q') => ⟨comp' e2 (next r) (ADD r c) , n ,p, q', s[r:=NUM n]⟩
-      | (None, q') => ⟪p, q', s⟫
+      | Some (n, q') => ⟨comp' e2 (next r) (ADD r c) , n ,p, q', s[r:=NUM n]⟩
+      | None => ⟪p, s⟫
       end.
   <== { apply vm_store }
       match eval e1 q with
-      | (Some n, q') => ⟨STORE r (comp' e2 (next r) (ADD r c)) , n ,p, q', s⟩
-      | (None, q') => ⟪p, q', s⟫
+      | Some (n, q') => ⟨STORE r (comp' e2 (next r) (ADD r c)) , n ,p, q', s⟩
+      | None => ⟪p, s⟫
       end.
   <|= { apply IHe1 }
     ⟨comp' e1 r (STORE r (comp' e2 (next r) (ADD r c))), a,p, q, s⟩.
@@ -205,11 +206,11 @@ Proof.
   
   begin
     match eval Throw q with
-    | (Some n, q') => ⟨c , n ,p, q', s⟩
-    | (None, q') => ⟪p, q', s⟫
+    | Some (n, q') => ⟨c , n ,p, q', s⟩
+    | None => ⟪p, s⟫
     end.
   = { auto }
-      ⟪p, q, s⟫.
+      ⟪p, s⟫.
   <== { apply vm_throw }
       ⟨THROW, a, p, q, s⟩.
   [].
@@ -218,44 +219,44 @@ Proof.
   
   begin
     match eval (Catch e1 e2) q with
-    | (Some n, q') => ⟨c , n ,p, q', s⟩
-    | (None, q') => ⟪p, q', s⟫
+    | Some (n, q') => ⟨c , n ,p, q', s⟩
+    | None => ⟪p, s⟫
     end.
   = { auto }
       match eval e1 q with
-      | (Some n, q') => ⟨c , n ,p, q', s⟩
-      | (None, q') => match eval e2 q' with
-                      | (Some n', q'') => ⟨c , n' ,p, q'', s⟩
-                      | (None, q'') => ⟪p, q'', s⟫
-                      end
+      | Some (n, q') => ⟨c , n ,p, q', s⟩
+      | None => match eval e2 q with
+                | Some (n', q'') => ⟨c , n' ,p, q'', s⟩
+                | None => ⟪p,s⟫
+                end
       end.
   <|= { apply IHe2 }
       match eval e1 q with
-      | (Some n, q') => ⟨c , n ,p, q', s⟩
-      | (None, q') => ⟨comp' e2  r c , 0 ,p, q', s⟩
+      | Some (n, q') => ⟨c, n ,p, q', s⟩
+      | None => ⟨comp' e2  r c , 0 ,p, q, s⟩
       end.
   ≤ { eauto }
       match eval e1 q with
-      | (Some n, q') => ⟨c , n ,p, q', s⟩
-      | (None, q') => ⟨comp' e2  r c , 0 ,p, q', s[r:= HAN (comp' e2  r c) p]⟩
+      | Some (n, q') => ⟨c , n ,p, q', s⟩
+      | None => ⟨comp' e2  r c , 0 ,p, q, s[r:= HAN (comp' e2  r c) p q]⟩
       end.
   <== {apply vm_fail}
       match eval e1 q with
-      | (Some n, q') => ⟨c , n ,p, q', s⟩
-      | (None, q') => ⟪Some r, q', s[r:= HAN (comp' e2  r c) p]⟫
+      | Some (n, q') => ⟨c , n ,p, q', s⟩
+      | None => ⟪Some r, s[r:= HAN (comp' e2  r c) p q]⟫
       end.
   ≤ {auto}
       match eval e1 q with
-      | (Some n, q') => ⟨c , n ,p, q', s[r:= HAN (comp' e2  r c) p]⟩
-      | (None, q') => ⟪Some r, q', s[r:= HAN (comp' e2  r c) p]⟫
+      | Some (n, q') => ⟨c , n ,p, q', s[r:= HAN (comp' e2  r c) p q]⟩
+      | None => ⟪Some r, s[r:= HAN (comp' e2  r c) p q]⟫
       end.
   <== {eapply vm_unmark}
       match eval e1 q with
-      | (Some n, q') => ⟨UNMARK c , n,Some r, q', s[r:= HAN (comp' e2  r c) p]⟩
-      | (None, q') => ⟪Some r, q', s[r:= HAN (comp' e2  r c) p]⟫
+      | Some (n, q') => ⟨UNMARK c , n,Some r, q', s[r:= HAN (comp' e2  r c) p q]⟩
+      | None => ⟪Some r, s[r:= HAN (comp' e2  r c) p q]⟫
       end.
   <|= {apply IHe1}
-      ⟨comp' e1 (next r) (UNMARK c) , a ,Some r, q, s[r:= HAN (comp' e2  r c) p]⟩.
+      ⟨comp' e1 (next r) (UNMARK c) , a ,Some r, q, s[r:= HAN (comp' e2  r c) p q]⟩.
   <== {apply vm_mark}
       ⟨MARK r (comp' e2  r c) (comp' e1 (next r) (UNMARK c)) , a ,p, q, s⟩.
   [].
@@ -263,8 +264,8 @@ Proof.
 
   begin
     match eval Get q with
-    | (Some n, q') => ⟨c , n ,p, q', s⟩
-    | (None, q') => ⟪p, q', s⟫
+    | Some (n, q') => ⟨c , n ,p, q', s⟩
+    | None => ⟪p, s⟫
     end.
   = {auto}
       ⟨c , q ,p, q, s⟩.
@@ -274,26 +275,26 @@ Proof.
   
   begin
     match eval (Put e1 e2) q with
-    | (Some n, q') => ⟨c , n ,p, q', s⟩
-    | (None, q') => ⟪p, q', s⟫
+    | Some (n, q') => ⟨c , n ,p, q', s⟩
+    | None => ⟪p, s⟫
     end.
   = {auto}
     match eval e1 q with
-    | (Some n, q') => match eval e2 n with
-                      | (Some n', q'') => ⟨c , n' ,p, q'', s⟩
-                      | (None, q'') => ⟪p, q'', s⟫
+    | Some (n, q') => match eval e2 n with
+                      | Some (n', q'') => ⟨c , n' ,p, q'', s⟩
+                      | None => ⟪p, s⟫
                       end
-    | (None, q') => ⟪p, q', s⟫
+    | None => ⟪p, s⟫
     end.
   <|= {apply IHe2}
     match eval e1 q with
-    | (Some n, q') => ⟨comp' e2 r c , n ,p, n, s⟩
-    | (None, q') => ⟪p, q', s⟫
+    | Some (n, q') => ⟨comp' e2 r c , n ,p, n, s⟩
+    | None => ⟪p, s⟫
     end.
   <== {apply vm_write}
     match eval e1 q with
-    | (Some n, q') => ⟨WRITE (comp' e2 r c) , n ,p, q', s⟩
-    | (None, q') => ⟪p, q', s⟫
+    | Some (n, q') => ⟨WRITE (comp' e2 r c) , n ,p, q', s⟩
+    | None => ⟪p, s⟫
     end.
   <|= {apply IHe1}
       ⟨comp' e1 r (WRITE (comp' e2 r c)) , a ,p, q, s⟩.
@@ -310,12 +311,12 @@ Qed.
 
 Lemma determ_vm : determ VM.
   intros C C1 C2 V. induction V; intro V'; inversion V'; subst;eauto.
-  rewrite H in *; dist. rewrite H in H4. dist. rewrite H in H6. dist.
+  rewrite H in *; dist. rewrite H in H3. dist. rewrite H in H6. dist.
 Qed.
 
 
 Theorem sound x a p q q' s n C :
-  freeFrom adr0 s -> eval x q = (Some n, q')
+  freeFrom adr0 s -> eval x q = Some (n, q')
   -> ⟨comp x, a, p, q, s⟩ =>>! C -> exists s', C = ⟨HALT, n,p, q', s'⟩.
 Proof.
   intros F E M.
@@ -329,4 +330,4 @@ Proof.
   inversion H3.
 Qed.
 
-End State.
+End LocalState.
